Adapted named list formalization

Isotope/Syntax/NamedList/Ctx.lean
@@ -39,78 +39,99 @@ theorem Var.le.rel {T} [HasLin T] {l r: Var T}
 --In this case can define separation-style judgements on domains...
 abbrev Ctx (T: Type u) := List (Var T)
 
+inductive Ctx.has_name {T: Type u}: Ctx T -> String -> Prop
+  | head (q n A) (Γ: Ctx T): Ctx.has_name (⟨q, n, A⟩::Γ) n
+  | tail v (Γ: Ctx T) (m: String): Ctx.has_name Γ m -> Ctx.has_name (v::Γ) m
+
 instance Ctx.instHasLin {T: Type u} [HasLin T]: HasLin (Ctx T) where
   aff Γ := Γ.all HasLin.aff
   rel Γ := Γ.all HasLin.rel
 
 inductive Ctx.split {T: Type u} [HasLin T]: Ctx T → Ctx T → Ctx T → Type u
   | nil: split [] [] []
-  | left {Γ Δ Ξ} (v l):  l ≤ v → split Γ Δ Ξ → split (v::Γ) (l::Δ) Ξ
-  | right {Γ Δ Ξ} (v r): r ≤ v → split Γ Δ Ξ → split (v::Γ) Δ (r::Ξ)
-  | discard {Γ Δ Ξ} (v): HasLin.aff v → split Γ Δ Ξ → split (v::Γ) Δ Ξ
-  | dup {Γ Δ Ξ} (v l r): HasLin.rel v → l ≤ v → r ≤ v → split Γ Δ Ξ
+  | left {Γ Δ Ξ} {v l}:  l ≤ v → split Γ Δ Ξ → split (v::Γ) (l::Δ) Ξ
+  | right {Γ Δ Ξ} {v r}: r ≤ v → split Γ Δ Ξ → split (v::Γ) Δ (r::Ξ)
+  | discard {Γ Δ Ξ} {v}: HasLin.aff v → split Γ Δ Ξ → split (v::Γ) Δ Ξ
+  | dup {Γ Δ Ξ} {v l r}: HasLin.rel v → l ≤ v → r ≤ v → split Γ Δ Ξ
     → split (v::Γ) (l::Δ) (r::Ξ)
 
-inductive Ctx.split.strict {T: Type u} [HasLin T]
-  : {Γ Δ Ξ: Ctx T} -> split Γ Δ Ξ -> Prop
-  | nil: strict nil
-  | left (v H): strict H → strict (left v v (le_refl v) H)
-  | right (v H): strict H → strict (right v v (le_refl v) H)
-  | dup (v Hr H)
-    : strict H → strict (dup v v v Hr (le_refl v) (le_refl v) H)
+@[match_pattern]
+def Ctx.split.sleft {T: Type u} [HasLin T] {Γ Δ Ξ: Ctx T}
+  (v: Var T): split Γ Δ Ξ -> split (v::Γ) (v::Δ) Ξ
+  := left (le_refl v)
+@[match_pattern]
+def Ctx.split.sright {T: Type u} [HasLin T] {Γ Δ Ξ: Ctx T}
+  (v: Var T): split Γ Δ Ξ -> split (v::Γ) Δ (v::Ξ)
+  := right (le_refl v)
+@[match_pattern]
+def Ctx.split.sdup {T: Type u} [HasLin T] {Γ Δ Ξ: Ctx T}
+  {v} (Hv: HasLin.rel v): split Γ Δ Ξ -> split (v::Γ) (v::Δ) (v::Ξ)
+  := dup Hv (le_refl v) (le_refl v)
 
 inductive Ctx.ssplit {T: Type u} [HasLin T]: Ctx T → Ctx T → Ctx T → Type u
   | nil: ssplit [] [] []
-  | left {Γ Δ Ξ} (v):  ssplit Γ Δ Ξ → ssplit (v::Γ) (v::Δ) Ξ
-  | right {Γ Δ Ξ} (v): ssplit Γ Δ Ξ → ssplit (v::Γ) Δ (v::Ξ)
-  | dup {Γ Δ Ξ} (v): HasLin.rel v → ssplit Γ Δ Ξ
-    → ssplit (v::Γ) (v::Δ) (v::Ξ)
+  | left {Γ Δ Ξ} {v l}:  l ≤ v → ssplit Γ Δ Ξ → ssplit (v::Γ) (l::Δ) Ξ
+  | right {Γ Δ Ξ} {v r}: r ≤ v → ssplit Γ Δ Ξ → ssplit (v::Γ) Δ (r::Ξ)
+  | dup {Γ Δ Ξ} {v l r}: HasLin.rel v → l ≤ v → r ≤ v → ssplit Γ Δ Ξ
+    → ssplit (v::Γ) (l::Δ) (r::Ξ)
+
+@[match_pattern]
+def Ctx.ssplit.sleft {T: Type u} [HasLin T] {Γ Δ Ξ: Ctx T}
+  (v: Var T): ssplit Γ Δ Ξ -> ssplit (v::Γ) (v::Δ) Ξ
+  := left (le_refl v)
+@[match_pattern]
+def Ctx.ssplit.sright {T: Type u} [HasLin T] {Γ Δ Ξ: Ctx T}
+  (v: Var T): ssplit Γ Δ Ξ -> ssplit (v::Γ) Δ (v::Ξ)
+  := right (le_refl v)
+@[match_pattern]
+def Ctx.ssplit.sdup {T: Type u} [HasLin T] {Γ Δ Ξ: Ctx T}
+  {v} (Hv: HasLin.rel v): ssplit Γ Δ Ξ -> ssplit (v::Γ) (v::Δ) (v::Ξ)
+  := dup Hv (le_refl v) (le_refl v)
 
 def Ctx.ssplit.toSplit {T: Type u} [HasLin T] {Γ Δ Ξ: Ctx T}
   : ssplit Γ Δ Ξ → split Γ Δ Ξ
   | nil => split.nil
-  | left v H => split.left v v (le_refl v) (ssplit.toSplit H)
-  | right v H => split.right v v (le_refl v) (ssplit.toSplit H)
-  | dup v Hr H =>
-    split.dup v v v Hr (le_refl v) (le_refl v) (ssplit.toSplit H)
+  | left Hl H => split.left Hl (ssplit.toSplit H)
+  | right Hr H => split.right Hr (ssplit.toSplit H)
+  | dup Hrel Hl Hr H => split.dup Hrel Hl Hr (ssplit.toSplit H)
 
 def Ctx.split.swap {T: Type u} [HasLin T] {Γ Δ Ξ: Ctx T}
   : split Γ Δ Ξ -> split Γ Ξ Δ
   | nil => nil
-  | left v l Hl H => right v l Hl (swap H)
-  | right v r Hl H => left v r Hl (swap H)
-  | discard v Ha Hl => discard v Ha (swap Hl)
-  | dup v l r H Hl Hr HΓ
-    => dup v r l H Hr Hl (swap HΓ)
+  | left Hl H => right Hl (swap H)
+  | right Hl H => left Hl (swap H)
+  | discard Ha Hl => discard Ha (swap Hl)
+  | dup H Hl Hr HΓ
+    => dup H Hr Hl (swap HΓ)
 
 def Ctx.ssplit.swap {T: Type u} [HasLin T] {Γ Δ Ξ: Ctx T}
   : ssplit Γ Δ Ξ -> ssplit Γ Ξ Δ
   | nil => nil
-  | left v H => right v (swap H)
-  | right v H => left v (swap H)
-  | dup v Hr H => dup v Hr (swap H)
+  | left Hl H => right Hl (swap H)
+  | right Hr H => left Hr (swap H)
+  | dup Hrel Hl Hr H => dup Hrel Hr Hl (swap H)
 
 def Ctx.ssplit.swap_toSplit {T: Type u} [HasLin T] {Γ Δ Ξ: Ctx T}
   : (H: ssplit Γ Δ Ξ) -> H.swap.toSplit = H.toSplit.swap
   | nil => rfl
-  | left v H => congrArg _ (swap_toSplit H)
-  | right v H => congrArg _ (swap_toSplit H)
-  | dup v Hr H => congrArg _ (swap_toSplit H)
+  | left _ H => congrArg _ (swap_toSplit H)
+  | right _ H => congrArg _ (swap_toSplit H)
+  | dup _ _ _ H => congrArg _ (swap_toSplit H)
 
 def Ctx.split.swap_idem {T: Type u} [HasLin T] {Γ Δ Ξ: Ctx T}
   : Function.LeftInverse (@swap T _ Γ Δ Ξ) (@swap T _ Γ Ξ Δ)
   | nil => rfl
-  | left v l Hl HΓ => by simp [swap, swap_idem HΓ]
-  | right v r Hr HΓ => by simp [swap, swap_idem HΓ]
-  | discard v Ha HΓ => by simp [swap, swap_idem HΓ]
-  | dup v l r Har Hl Hr HΓ => by simp [swap, swap_idem HΓ]
+  | left _ HΓ => by simp [swap, swap_idem HΓ]
+  | right _ HΓ => by simp [swap, swap_idem HΓ]
+  | discard _ HΓ => by simp [swap, swap_idem HΓ]
+  | dup _ _ _ HΓ => by simp [swap, swap_idem HΓ]
 
 def Ctx.ssplit.swap_idem {T: Type u} [HasLin T] {Γ Δ Ξ: Ctx T}
   : Function.LeftInverse (@swap T _ Γ Δ Ξ) (@swap T _ Γ Ξ Δ)
   | nil => rfl
-  | left v H => by simp [swap, swap_idem H]
-  | right v H => by simp [swap, swap_idem H]
-  | dup v Hr H => by simp [swap, swap_idem H]
+  | left _ H => by simp [swap, swap_idem H]
+  | right _ H => by simp [swap, swap_idem H]
+  | dup _ _ _ H => by simp [swap, swap_idem H]
 
 def Ctx.split.swap_equiv {T: Type u} [HasLin T] (Γ Δ Ξ: Ctx T)
   : Equiv (split Γ Δ Ξ) (split Γ Ξ Δ) where
@@ -129,10 +150,10 @@ def Ctx.ssplit.swap_equiv {T: Type u} [HasLin T] (Γ Δ Ξ: Ctx T)
 theorem Ctx.split.left_length_decreasing {T: Type u} [HasLin T] {Γ Δ Ξ: Ctx T}
   : split Γ Δ Ξ -> Δ.length ≤ Γ.length
   | nil => le_refl _
-  | left _ _ _ HΓ => Nat.succ_le_succ HΓ.left_length_decreasing
-  | right _ _ _ HΓ => Nat.le_step HΓ.left_length_decreasing
-  | discard _ _ HΓ => Nat.le_step HΓ.left_length_decreasing
-  | dup _ _ _ _ _ _ HΓ => Nat.succ_le_succ HΓ.left_length_decreasing
+  | left _ HΓ => Nat.succ_le_succ HΓ.left_length_decreasing
+  | right _ HΓ => Nat.le_step HΓ.left_length_decreasing
+  | discard _ HΓ => Nat.le_step HΓ.left_length_decreasing
+  | dup _ _ _ HΓ => Nat.succ_le_succ HΓ.left_length_decreasing
 
 theorem Ctx.ssplit.left_length_decreasing {T: Type u} [HasLin T] {Γ Δ Ξ: Ctx T}
   (H: ssplit Γ Δ Ξ): Δ.length ≤ Γ.length
@@ -147,102 +168,107 @@ theorem Ctx.ssplit.right_length_decreasing {T: Type u} [HasLin T] {Γ Δ Ξ: Ctx
   := H.toSplit.right_length_decreasing
 
 def Ctx.wk {T: Type u} [HasLin T] (Γ Δ: Ctx T) := Ctx.split Γ Δ []
-
 def Ctx.var {T: Type u} [HasLin T] (Γ: Ctx T) (x: Var T) := Ctx.wk Γ [x]
 
 @[match_pattern]
 def Ctx.wk.nil {T: Type u} [HasLin T]: @Ctx.wk T _ [] [] := Ctx.split.nil
 @[match_pattern]
 def Ctx.wk.cons {T: Type u} [HasLin T] {Γ Δ: Ctx T}
-  : (v l: Var T) -> (Hl: l ≤ v) -> Ctx.wk Γ Δ -> Ctx.wk (v::Γ) (l::Δ)
+  : {v l: Var T} -> (Hl: l ≤ v) -> Ctx.wk Γ Δ -> Ctx.wk (v::Γ) (l::Δ)
   := Ctx.split.left
   @[match_pattern]
 def Ctx.wk.scons {T: Type u} [HasLin T] {Γ Δ: Ctx T}
   (v: Var T): Ctx.wk Γ Δ -> Ctx.wk (v::Γ) (v::Δ)
-  := Ctx.split.left v v (le_refl v)
+  := Ctx.split.left (le_refl v)
 @[match_pattern]
 def Ctx.wk.discard {T: Type u} [HasLin T] {Γ Δ: Ctx T}
-  : (v: Var T) -> (Ha: HasLin.aff v) -> Ctx.wk Γ Δ -> Ctx.wk (v::Γ) Δ
+  : {v: Var T} -> (Ha: HasLin.aff v) -> Ctx.wk Γ Δ -> Ctx.wk (v::Γ) Δ
   := Ctx.split.discard
+
+@[match_pattern]
+def Ctx.var.head {T: Type u} [HasLin T] {Γ: Ctx T}
+  {v v': Var T} (H: v ≥ v') (W: Γ.wk []): Ctx.var (v::Γ) v'
+  := Ctx.wk.cons H W
+@[match_pattern]
+def Ctx.var.shead {T: Type u} [HasLin T] {Γ: Ctx T}
+  (v: Var T) (W: Γ.wk []): Ctx.var (v::Γ) v
+  := Ctx.wk.scons v W
+@[match_pattern]
+def Ctx.var.tail {T: Type u} [HasLin T] {Γ: Ctx T}
+  {v a: Var T} (W: Γ.var v) (Ha: HasLin.aff a): Ctx.var (a::Γ) v
+  := Ctx.wk.discard Ha W
 
 def Ctx.split.left_decompose {T: Type u} [HasLin T] {Γ Δ Ξ: Ctx T}
   : Ctx.split Γ Δ Ξ
-  -> (Δ' Ξ': Ctx T) × Ctx.ssplit Γ Δ' Ξ' × Ctx.wk Δ' Δ × Ctx.wk Ξ' Ξ
-  | nil => ⟨[], [], ssplit.nil, wk.nil, wk.nil⟩
-  | left v l Hl H => let ⟨Δ', Ξ', HΓ, HΔ, HΞ⟩ := left_decompose H;
-    ⟨v::Δ', Ξ', ssplit.left v HΓ, wk.cons v l Hl HΔ, HΞ⟩
-  | right v r Hl H => let ⟨Δ', Ξ', HΓ, HΔ, HΞ⟩ := left_decompose H;
-    ⟨Δ', v::Ξ', ssplit.right v HΓ, HΔ, wk.cons v r Hl HΞ⟩
-  | discard v Ha H => let ⟨Δ', Ξ', HΓ, HΔ, HΞ⟩ := left_decompose H;
-    ⟨v::Δ', Ξ', ssplit.left v HΓ, wk.discard v Ha HΔ, HΞ⟩
-  | dup v l r Hrel Hl Hr H => let ⟨Δ', Ξ', HΓ, HΔ, HΞ⟩ := left_decompose H;
-    ⟨v::Δ', v::Ξ', ssplit.dup v Hrel HΓ, wk.cons v l Hl HΔ, wk.cons v r Hr HΞ⟩
+  -> (Δ': Ctx T) × Ctx.ssplit Γ Δ' Ξ × Ctx.wk Δ' Δ
+  | nil => ⟨[], ssplit.nil, wk.nil⟩
+  | left Hl H => let ⟨Δ', HΓ, HΔ⟩ := left_decompose H;
+    ⟨_::Δ', ssplit.left Hl HΓ, wk.scons _ HΔ⟩
+  | right Hr H => let ⟨Δ', HΓ, HΔ⟩ := left_decompose H;
+    ⟨Δ', ssplit.right Hr HΓ, HΔ⟩
+  | discard Ha H => let ⟨Δ', HΓ, HΔ⟩ := left_decompose H;
+    ⟨_::Δ', ssplit.sleft _ HΓ, wk.discard Ha HΔ⟩
+  | dup Hrel Hl Hr H => let ⟨Δ', HΓ, HΔ⟩ := left_decompose H;
+    ⟨_::Δ', ssplit.dup Hrel Hl Hr HΓ, wk.scons _ HΔ⟩
 
 def Ctx.split.right_decompose {T: Type u} [HasLin T] {Γ Δ Ξ: Ctx T}
   : Ctx.split Γ Δ Ξ
-  -> (Δ' Ξ': Ctx T) × Ctx.ssplit Γ Δ' Ξ' × Ctx.wk Δ' Δ × Ctx.wk Ξ' Ξ
-  | nil => ⟨[], [], ssplit.nil, wk.nil, wk.nil⟩
-  | left v l Hl H => let ⟨Δ', Ξ', HΓ, HΔ, HΞ⟩ := right_decompose H;
-    ⟨v::Δ', Ξ', ssplit.left v HΓ, wk.cons v l Hl HΔ, HΞ⟩
-  | right v r Hl H => let ⟨Δ', Ξ', HΓ, HΔ, HΞ⟩ := right_decompose H;
-    ⟨Δ', v::Ξ', ssplit.right v HΓ, HΔ, wk.cons v r Hl HΞ⟩
-  | discard v Ha H => let ⟨Δ', Ξ', HΓ, HΔ, HΞ⟩ := right_decompose H;
-    ⟨Δ', v::Ξ', ssplit.right v HΓ, HΔ, wk.discard v Ha HΞ⟩
-  | dup v l r Hrel Hl Hr H => let ⟨Δ', Ξ', HΓ, HΔ, HΞ⟩ := right_decompose H;
-    ⟨v::Δ', v::Ξ', ssplit.dup v Hrel HΓ, wk.cons v l Hl HΔ, wk.cons v r Hr HΞ⟩
+  -> (Ξ': Ctx T) × Ctx.ssplit Γ Δ Ξ' × Ctx.wk Ξ' Ξ
+  | nil => ⟨[], ssplit.nil, wk.nil⟩
+  | left Hl H => let ⟨Ξ', HΓ, HΞ⟩ := right_decompose H;
+    ⟨Ξ', ssplit.left Hl HΓ, HΞ⟩
+  | right Hr H => let ⟨Ξ', HΓ, HΞ⟩ := right_decompose H;
+    ⟨_::Ξ', ssplit.right Hr HΓ, wk.scons _ HΞ⟩
+  | discard Ha H => let ⟨Ξ', HΓ, HΞ⟩ := right_decompose H;
+    ⟨_::Ξ', ssplit.right (le_refl _) HΓ, wk.discard Ha HΞ⟩
+  | dup Hrel Hl Hr H => let ⟨Ξ', HΓ, HΞ⟩ := right_decompose H;
+    ⟨_::Ξ', ssplit.dup Hrel Hl Hr HΓ, wk.scons _ HΞ⟩
 
---TODO: adjust types here
 def Ctx.ssplit.distribute_left {T: Type u} [HasLin T] {Γ Γ' Δ Ξ: Ctx T}
   : Ctx.wk Γ' Γ -> Ctx.ssplit Γ Δ Ξ
-    -> (Δ' Ξ': Ctx T) × Ctx.ssplit Γ' Δ' Ξ' × Ctx.wk Δ' Δ × Ctx.wk Ξ' Ξ
-  | wk.nil, nil => ⟨[], [], ssplit.nil, wk.nil, wk.nil⟩
-  | wk.cons _ _ Hl W, left _ S =>
-    let ⟨_, _, HΓ, HΔ, HΞ⟩ := distribute_left W S;
-    ⟨_, _,
-      ssplit.left _ HΓ,
-      wk.cons _ _ Hl HΔ,
-      HΞ⟩
-  | wk.cons _ _ Hl W, right _ S =>
-    let ⟨_, _, HΓ, HΔ, HΞ⟩ := distribute_left W S;
-    ⟨_, _,
-      ssplit.right _ HΓ,
-      HΔ,
-      wk.cons _ _ Hl HΞ⟩
-  | wk.cons _ _ Hl W, dup _ Hrel S =>
-    let ⟨_, _, HΓ, HΔ, HΞ⟩ := distribute_left W S;
-    ⟨_, _,
-      ssplit.dup _ (Var.le.rel Hl Hrel) HΓ,
-      wk.cons _ _ Hl HΔ,
-      wk.cons _ _ Hl HΞ⟩
-  | wk.discard v Ha W, S =>
-    let ⟨_, _, HΓ, HΔ, HΞ⟩ := distribute_left W S;
-    ⟨_, _, left _ HΓ, wk.discard v Ha HΔ, HΞ⟩
+    -> (Δ': Ctx T) × Ctx.ssplit Γ' Δ' Ξ × Ctx.wk Δ' Δ
+  | wk.nil, nil => ⟨[], ssplit.nil, wk.nil⟩
+  | wk.cons Hc W, left Hl S =>
+    let ⟨_, HΓ, HΔ⟩ := distribute_left W S;
+    ⟨_,
+      ssplit.left (le_trans Hl Hc) HΓ,
+      wk.scons _ HΔ⟩
+  | wk.cons Hc W, right Hr S =>
+    let ⟨_, HΓ, HΔ⟩ := distribute_left W S;
+    ⟨_,
+      ssplit.right (le_trans Hr Hc) HΓ,
+      HΔ⟩
+  | wk.cons Hc W, dup Hrel Hl Hr S =>
+    let ⟨_, HΓ, HΔ⟩ := distribute_left W S;
+    ⟨_,
+      ssplit.dup (Var.le.rel Hc Hrel) (le_trans Hl Hc) (le_trans Hr Hc) HΓ,
+      wk.scons _ HΔ⟩
+  | wk.discard Ha W, S =>
+    let ⟨_, HΓ, HΔ⟩ := distribute_left W S;
+    ⟨_, sleft _ HΓ, wk.discard Ha HΔ⟩
 
 def Ctx.ssplit.distribute_right {T: Type u} [HasLin T] {Γ Γ' Δ Ξ: Ctx T}
   : Ctx.wk Γ' Γ -> Ctx.ssplit Γ Δ Ξ
-    -> (Δ' Ξ': Ctx T) × Ctx.ssplit Γ' Δ' Ξ' × Ctx.wk Δ' Δ × Ctx.wk Ξ' Ξ
-  | wk.nil, nil => ⟨[], [], ssplit.nil, wk.nil, wk.nil⟩
-  | wk.cons _ _ Hl W, left _ S =>
-    let ⟨_, _, HΓ, HΔ, HΞ⟩ := distribute_right W S;
-    ⟨_, _,
-      ssplit.left _ HΓ,
-      wk.cons _ _ Hl HΔ,
+    -> (Ξ': Ctx T) × Ctx.ssplit Γ' Δ Ξ' × Ctx.wk Ξ' Ξ
+  | wk.nil, nil => ⟨[], ssplit.nil, wk.nil⟩
+  | wk.cons Hc W, left Hl S =>
+    let ⟨_, HΓ, HΞ⟩ := distribute_right W S;
+    ⟨_,
+      ssplit.left (le_trans Hl Hc) HΓ,
       HΞ⟩
-  | wk.cons _ _ Hl W, right _ S =>
-    let ⟨_, _, HΓ, HΔ, HΞ⟩ := distribute_right W S;
-    ⟨_, _,
-      ssplit.right _ HΓ,
-      HΔ,
-      wk.cons _ _ Hl HΞ⟩
-  | wk.cons _ _ Hl W, dup _ Hrel S =>
-    let ⟨_, _, HΓ, HΔ, HΞ⟩ := distribute_right W S;
-    ⟨_, _,
-      ssplit.dup _ (Var.le.rel Hl Hrel) HΓ,
-      wk.cons _ _ Hl HΔ,
-      wk.cons _ _ Hl HΞ⟩
-  | wk.discard v Ha W, S =>
-    let ⟨_, _, HΓ, HΔ, HΞ⟩ := distribute_right W S;
-    ⟨_, _, right _ HΓ, HΔ, wk.discard v Ha HΞ⟩
+  | wk.cons Hc W, right Hr S =>
+    let ⟨_, HΓ, HΞ⟩ := distribute_right W S;
+    ⟨_,
+      ssplit.right (le_trans Hr Hc) HΓ,
+      wk.scons _ HΞ⟩
+  | wk.cons Hc W, dup Hrel Hl Hr S =>
+    let ⟨_, HΓ, HΞ⟩ := distribute_right W S;
+    ⟨_,
+      ssplit.dup (Var.le.rel Hc Hrel) (le_trans Hl Hc) (le_trans Hr Hc) HΓ,
+      wk.scons _ HΞ⟩
+  | wk.discard Ha W, S =>
+    let ⟨_, HΓ, HΞ⟩ := distribute_right W S;
+    ⟨_, sright _ HΓ, wk.discard Ha HΞ⟩
 
 theorem Ctx.wk.length_decreasing {T: Type u} [HasLin T] {Γ Δ: Ctx T} (H: wk Γ Δ)
   : Δ.length ≤ Γ.length
@@ -259,7 +285,7 @@ theorem Ctx.wk.nil_nil {T: Type u} [HasLin T] {Γ: Ctx T}
 def Ctx.wk.id {T: Type u} [HasLin T]
   : (Γ: Ctx T) -> Ctx.wk Γ Γ
   | [] => Ctx.split.nil
-  | v::Γ => Ctx.split.left v v (le_refl v) (id Γ)
+  | v::Γ => Ctx.split.left (le_refl v) (id Γ)
 
 instance Ctx.wk.instInhabitedRefl {T: Type u} [HasLin T] {Γ: Ctx T}
   : Inhabited (Ctx.wk Γ Γ) where
@@ -270,8 +296,8 @@ instance Ctx.wk.instSubsingletonRefl {T: Type u} [HasLin T] {Γ: Ctx T}
   allEq := let rec allEq
   : ∀ {Γ: Ctx T} (HΓ: Ctx.wk Γ Γ) (HΓ': Ctx.wk Γ Γ), HΓ = HΓ'
   | [], nil, nil => rfl
-  | _, cons _ _ _ HΓ, cons _ _ _ HΓ' => congrArg _ (allEq HΓ HΓ')
-  | _, discard _ _ HΓ, _ | _, _, discard _ _ HΓ => HΓ.append_false.elim
+  | _, cons _ HΓ, cons _ HΓ' => congrArg _ (allEq HΓ HΓ')
+  | _, discard _ HΓ, _ | _, _, discard _ HΓ => HΓ.append_false.elim
   allEq
 
 --TODO: subsingleton to nil --> nil is terminal object
@@ -280,26 +306,26 @@ instance Ctx.wk.instSubsingletonRefl {T: Type u} [HasLin T] {Γ: Ctx T}
 def Ctx.wk.comp {T: Type u} [HasLin T] {Γ Δ Ξ: Ctx T}
   : Ctx.wk Γ Δ -> Ctx.wk Δ Ξ -> Ctx.wk Γ Ξ
   | nil, nil => nil
-  | cons _ _ Hl HΓ, cons _ _ Hl' HΓ' =>
-    cons _ _ (le_trans Hl' Hl) (comp HΓ HΓ')
-  | cons _ _ Hl HΓ, discard _ Ha HΓ' =>
-    discard _ (Var.le.aff Hl Ha) (comp HΓ HΓ')
-  | discard _ Ha HΓ, H =>
-    discard _ Ha (comp HΓ H)
+  | cons Hl HΓ, cons Hl' HΓ' =>
+    cons (le_trans Hl' Hl) (comp HΓ HΓ')
+  | cons Hl HΓ, discard Ha HΓ' =>
+    discard (Var.le.aff Hl Ha) (comp HΓ HΓ')
+  | discard Ha HΓ, H =>
+    discard Ha (comp HΓ H)
 
 def Ctx.wk.comp_id {T: Type u} [HasLin T] {Γ Δ: Ctx T}
   : (H: Ctx.wk Γ Δ) -> (R: Ctx.wk Δ Δ) -> H.comp R = H
   | nil, nil => rfl
-  | cons _ _ _ HΓ, cons _ _ _ HΓ' => congrArg _ (comp_id HΓ HΓ')
-  | discard _ _ HΓ, HΓ' => congrArg _ (comp_id HΓ HΓ')
-  | cons _ _ _ _, discard _ _ HΓ => HΓ.append_false.elim
+  | cons _ HΓ, cons _ HΓ' => congrArg _ (comp_id HΓ HΓ')
+  | discard _ HΓ, HΓ' => congrArg _ (comp_id HΓ HΓ')
+  | cons _ _, discard _ HΓ => HΓ.append_false.elim
 
 def Ctx.wk.id_comp {T: Type u} [HasLin T] {Γ Δ: Ctx T}
   : (R: Ctx.wk Γ Γ) -> (H: Ctx.wk Γ Δ) -> R.comp H = H
   | nil, nil => rfl
-  | cons _ _ _ HΓ, cons _ _ _ HΓ' => congrArg _ (id_comp HΓ HΓ')
-  | cons _ _ _ HΓ, discard _ _ HΓ' => congrArg _ (id_comp HΓ HΓ')
-  | discard _ _ HΓ, _ => HΓ.append_false.elim
+  | cons _ HΓ, cons _ HΓ' => congrArg _ (id_comp HΓ HΓ')
+  | cons _ HΓ, discard _ HΓ' => congrArg _ (id_comp HΓ HΓ')
+  | discard _ HΓ, _ => HΓ.append_false.elim
 
 def Ctx.wk.comp_assoc {T: Type u} [HasLin T] {Γ Δ Ξ Θ: Ctx T}
   : (X: Ctx.wk Γ Δ)
@@ -307,23 +333,23 @@ def Ctx.wk.comp_assoc {T: Type u} [HasLin T] {Γ Δ Ξ Θ: Ctx T}
   -> (Z: Ctx.wk Ξ Θ)
   -> (X.comp Y).comp Z = X.comp (Y.comp Z)
   | nil, nil, nil => rfl
-  | cons _ _ _ X, cons _ _ _ Y, cons _ _ _ Z => congrArg _ (comp_assoc X Y Z)
-  | cons _ _ _ X, cons _ _ _ Y, discard _ _ Z => congrArg _ (comp_assoc X Y Z)
-  | cons _ _ _ X, discard _ _ Y, Z => congrArg _ (comp_assoc X Y Z)
-  | discard _ _ X, Y, Z => congrArg _ (comp_assoc X Y Z)
+  | cons _ X, cons _ Y, cons _ Z => congrArg _ (comp_assoc X Y Z)
+  | cons _ X, cons _ Y, discard _ Z => congrArg _ (comp_assoc X Y Z)
+  | cons _ X, discard _ Y, Z => congrArg _ (comp_assoc X Y Z)
+  | discard _ X, Y, Z => congrArg _ (comp_assoc X Y Z)
 
 def Ctx.wk.antisymm {T: Type u} [HasLin T] {Γ Δ: Ctx T}
   : Ctx.wk Γ Δ -> Ctx.wk Δ Γ -> Γ = Δ
   | nil, nil => rfl
-  | cons _ _ Hl HΓ, cons _ _ Hl' HΓ' =>
+  | cons Hl HΓ, cons Hl' HΓ' =>
     by rw [antisymm HΓ HΓ', le_antisymm Hl Hl']
-  | cons _ _ _ HΓ, discard _ _ HΓ' =>
+  | cons _ HΓ, discard _ HΓ' =>
     have H := le_trans HΓ'.length_decreasing HΓ.length_decreasing;
     by simp_arith at H
-  | discard _ _ HΓ, cons _ _ _ HΓ' =>
+  | discard _ HΓ, cons _ HΓ' =>
     have H := le_trans HΓ.length_decreasing HΓ'.length_decreasing;
     by simp_arith at H
-  | discard _ _ HΓ, discard _ _ HΓ' =>
+  | discard _ HΓ, discard _ HΓ' =>
     have H := le_trans (Nat.le_step HΓ'.length_decreasing) HΓ.length_decreasing;
     by simp_arith at H
 
@@ -346,4 +372,4 @@ def Ctx.wk.equiv_right {T: Type u} [HasLin T] {Γ Δ: Ctx T}
 
 def Ctx.var.upgrade {T: Type u} [HasLin T] {Γ: Ctx T} {v v': Var T}
   (H: Γ.var v) (H': v ≥ v'): Γ.var v'
-  := Ctx.wk.comp H (Ctx.wk.cons v v' H' (Ctx.wk.nil))
+  := Ctx.wk.comp H (Ctx.wk.cons H' (Ctx.wk.nil))
